spc/IPM.v
@@ -192,13 +192,28 @@ Section IPM.
     rr. uipropall. i. rr in H. uipropall. des. eapply iProp_mono; eauto.
     exists a. rewrite H. r_solve.
   Qed.
-
+  
+  Global Instance iProp_affine (P: iProp): Affine P.
+  Proof.
+    rr. uipropall. i. rr. uipropall.
+  Qed.
   Global Instance iProp_pure_forall: BiPureForall iProp.
   Proof.
     ii. rr. uipropall. i. rr. rr in H. uipropall.
     i. specialize (H a). rr in H. uipropall.
   Qed.
-End IPM.
+
+  Global Instance iProp_bi_affine : BiAffine (iProp) | 0.
+  Proof. exact iProp_affine. Qed.
+
+  Global Instance iProp_bi_persistently_forall : BiPersistentlyForall iProp.
+  Proof.
+    ii. rr. uipropall. i. rr. rr in H. uipropall.
+    i. rr. uipropall. i. specialize (H x). rr in H. uipropall.
+  Qed.
+
+  End IPM.
+Global Hint Immediate iProp_bi_affine : core.
 Arguments OwnM: simpl never.
 
 Section TEST.
@@ -221,6 +236,59 @@ Infix "⊢" := (@bi_entails iProp).
 Infix "**" := bi_sep (at level 99).
 Infix "-*" := bi_wand (at level 99, right associativity).
 Notation "#=> P" := ((@bupd (bi_car (@iProp _)) (@bi_bupd_bupd (@iProp _) (@iProp_bi_bupd _))) P) (at level 99).
+
+Section IUPD.
+  Context {Σ: GRA.t}.
+
+  Definition IUpd (I: iProp): iProp -> iProp :=
+    fun P => I -* #=> (I ** P).
+
+  Lemma IUpd_intro I: forall P, P ⊢ IUpd I P.
+  Proof.
+    ii. iIntros "H INV". iModIntro. iFrame.
+  Qed.
+
+  Lemma IUpd_mono I: forall P Q, (P ⊢ Q) -> (IUpd I P ⊢ IUpd I Q).
+  Proof.
+    ii. unfold IUpd. iIntros "H INV".
+    iPoseProof ("H" with "INV") as "> [H0 H1]". iModIntro.
+    iFrame. iApply H. auto.
+  Qed.
+
+  Lemma IUpd_trans I: forall P, (IUpd I (IUpd I P)) ⊢ (IUpd I P).
+  Proof.
+    ii. unfold IUpd. iIntros "H INV".
+    iPoseProof ("H" with "INV") as "> [H0 H1]".
+    iApply "H1". auto.
+  Qed.
+
+  Lemma IUpd_frame_r I: forall P R, ((IUpd I P) ** R) ⊢ (IUpd I (P ** R)).
+  Proof.
+    ii. unfold IUpd. iIntros "[H0 H1] INV".
+    iPoseProof ("H0" with "INV") as "> [H0 H2]".
+    iModIntro. iFrame.
+  Qed.
+
+  Lemma Upd_IUpd I: forall P, #=> P ⊢ (IUpd I P).
+  Proof.
+    ii. unfold IUpd. iIntros "H INV". iFrame.
+  Qed.
+
+  Lemma iProp_bupd_mixin_IUpd I: BiBUpdMixin iProp (IUpd I).
+  Proof.
+    econs.
+    - ii. unfold bupd. unfold IUpd. rewrite H. auto.
+    - apply IUpd_intro.
+    - apply IUpd_mono.
+    - apply IUpd_trans.
+    - apply IUpd_frame_r.
+  Qed.
+  Global Instance iProp_bi_bupd_IUpd I: BiBUpd iProp := {| bi_bupd_mixin := iProp_bupd_mixin_IUpd I |}.
+End IUPD.
+Notation "#=( Q )=> P" := ((@bupd (bi_car (@iProp _)) (@bi_bupd_bupd (@iProp _) (@iProp_bi_bupd_IUpd _ Q))) P) (at level 99).
+Notation "P =( I ) =∗ Q" := (P ⊢ #=( I )=> Q) (only parsing, at level 99) : stdpp_scope.
+Notation "P =( I )=∗ Q" := (P -∗ #=( I )=> Q)%I (at level 99): bi_scope.
+
 
 Class IsOp {A : URA.t} (a b1 b2 : A) := is_op : a = b1 ⋅ b2.
 Global Arguments is_op {_} _ _ _ {_}.
@@ -338,23 +406,19 @@ Section ILEMMAS.
     rr. uipropall. i. rr. uipropall. des. rr in H. uipropall.
   Qed.
 
-  (*** this is deprecated in 1.1 ***)
-  (* Lemma Own_Upd_set *)
-  (*       (r1: Σ) B *)
-  (*       (UPD: URA.updatable_set r1 B) *)
-  (*   : *)
-  (*     (Own r1) ⊢ (#=> (∃ b, ⌜B b⌝ ** (Own b))) *)
-  (* . *)
-  (* Proof. *)
-  (*   cut (Entails (Own r1) (Upd (Ex (fun b => Sepconj (Pure (B b)) (Own b))))); ss. *)
-  (*   uipropall. i. red in H. des. subst. *)
-  (*   exploit (UPD (ctx0 ⋅ ctx)). *)
-  (*   { rewrite URA.add_assoc. et. } *)
-  (*   i. des. exists (b ⋅ ctx0). split. *)
-  (*   { rewrite <- URA.add_assoc. et. } *)
-  (*   { exists b. uipropall. esplits; [|apply IN|refl]. *)
-  (*     eapply URA.add_comm. } *)
-  (* Qed. *)
+  Lemma Own_Upd_set
+        (r1: Σ) B
+        (UPD: URA.updatable_set r1 B)
+    :
+      (Own r1) ⊢ (#=> (∃ b, ⌜B b⌝ ** (Own b)))
+  .
+  Proof.
+    destruct UPD. des.
+    cut (Entails (Own r1) (Upd (Ex (fun b => Sepconj (Pure (B b)) (Own b))))); ss.
+    uipropall. i. esplits; cycle 1.
+    { i. instantiate (1:= x). eapply H0. eapply URA.wf_extends; et. eapply URA.extends_add. et. }
+    uipropall. exists ε, x. esplits; et; [r_solve|refl]. 
+  Qed.
 
   Lemma Own_Upd
         (r1 r2: Σ)
@@ -377,45 +441,62 @@ Section ILEMMAS.
     red. uipropall. ii. etrans; et.
   Qed.
 
-  (*** this is deprecated in 1.1 ***)
-  (* Lemma OwnM_Upd_set (M: URA.t) `{@GRA.inG M Σ} *)
-  (*       (r1: M) B *)
-  (*       (UPD: URA.updatable_set r1 B) *)
-  (*   : *)
-  (*     (OwnM r1) ⊢ (#=> (∃ b, ⌜B b⌝ ** (OwnM b))) *)
-  (* . *)
-  (* Proof. *)
-  (*   assert (UPDM: URA.updatable_set *)
-  (*                   (GRA.embed r1) *)
-  (*                   (fun r => exists m, r = GRA.embed m /\ B m)). *)
-  (*   { red. i. red in UPD. *)
-  (*     unshelve hexploit UPD. *)
-  (*     { eapply (@eq_rect URA.t (Σ (@GRA.inG_id _ _ H)) (@URA.car)). *)
-  (*       { eapply (ctx (@GRA.inG_id _ _ H)). } *)
-  (*       { symmetry. eapply (@GRA.inG_prf _ _ H). } *)
-  (*     } *)
-  (*     Local Transparent GRA.to_URA. *)
-  (*     { ur in WF. ss. specialize (WF GRA.inG_id). *)
-  (*       destruct H. subst. ss. *)
-  (*       unfold GRA.embed in WF. ss. *)
-  (*       replace (PeanoNat.Nat.eq_dec inG_id inG_id) *)
-  (*         with (@left (inG_id = inG_id) (inG_id <> inG_id) eq_refl) in WF; ss. *)
-  (*       { des_ifs. repeat f_equal. eapply proof_irrelevance. } *)
-  (*     } *)
-  (*     i. des. exists (GRA.embed b). esplits; et. *)
-  (*     ur. Local Transparent GRA.to_URA. ss. *)
-  (*     i. unfold GRA.embed. des_ifs. *)
-  (*     { ss. unfold PCM.GRA.cast_ra. destruct  H. subst. ss. } *)
-  (*     { ur in WF. specialize (WF k). rewrite URA.unit_idl. *)
-  (*       eapply URA.wf_mon. rewrite URA.add_comm. et. *)
-  (*     } *)
-  (*   } *)
-  (*   iIntros "H". *)
-  (*   iPoseProof (Own_Upd_set with "H") as "> H". *)
-  (*   { eapply UPDM. } *)
-  (*   iDestruct "H" as (b) "[% H1]". des. subst. *)
-  (*   iModIntro. iExists m. iFrame. ss. *)
-  (* Qed. *)
+  Lemma Own_persistently (r : Σ) : Own r ⊢ <pers> Own (URA.core r).
+  Proof.
+    uipropall. i. rr; uipropall. apply URA.extends_core. ss.
+  Qed.
+
+  Lemma OwnM_persistently {M : URA.t} `{@GRA.inG M Σ} (r : M) : OwnM r ⊢ <pers> OwnM (URA.core r).
+  Proof.
+    unfold OwnM. rewrite GRA.embed_core. apply Own_persistently.
+  Qed.
+
+  Lemma OwnM_unit {M : URA.t} `{@GRA.inG M Σ} : ⊢ OwnM ε.
+  Proof.
+    Local Transparent GRA.to_URA.
+    rr; uipropall. i. rr; uipropall. rr. exists r.
+    rewrite GRA.embed_unit. rewrite URA.unit_idl. ss.
+  Qed.
+
+  Lemma OwnM_Upd_set (M: URA.t) `{@GRA.inG M Σ}
+        (r1: M) B
+        (UPD: URA.updatable_set r1 B)
+    :
+      (OwnM r1) ⊢ (#=> (∃ b, ⌜B b⌝ ** (OwnM b)))
+  .
+  Proof.
+    assert (UPDM: URA.updatable_set
+                    (GRA.embed r1)
+                    (fun r => exists m, r = GRA.embed m /\ B m)).
+    {
+      destruct UPD. des. r.
+      exists (GRA.embed x). esplits; et. i.
+      unshelve hexploit H1.
+      { eapply (@eq_rect URA.t (Σ (@GRA.inG_id _ _ H)) (@URA.car)).
+        { eapply (ctx (@GRA.inG_id _ _ H)). }
+        { symmetry. eapply (@GRA.inG_prf _ _ H). }
+      }
+      Local Transparent GRA.to_URA.
+      { ur in WF. ss. specialize (WF GRA.inG_id).
+        destruct H. subst. ss.
+        unfold GRA.embed in WF. ss.
+        replace (PeanoNat.Nat.eq_dec inG_id inG_id)
+          with (@left (inG_id = inG_id) (inG_id <> inG_id) eq_refl) in WF; ss.
+        { des_ifs. repeat f_equal. eapply proof_irrelevance. }
+      }
+      i. ur. Local Transparent GRA.to_URA. ss.
+      i. unfold GRA.embed. des_ifs.
+      { ss. unfold PCM.GRA.cast_ra. destruct  H. subst. ss. }
+      { ur in WF. specialize (WF k). rewrite URA.unit_idl.
+        eapply URA.wf_mon. rewrite URA.add_comm. eauto.
+      }
+    }
+    iIntros "H".
+    iPoseProof (Own_Upd_set with "H") as "> H".
+    { eapply UPDM. }
+    iDestruct "H" as (b) "[% H1]". des. subst.
+    iModIntro. iExists m. iFrame. ss.
+  Qed.
 
   Lemma OwnM_Upd (M: URA.t) `{@GRA.inG M Σ}
         (r1 r2: M)
@@ -441,8 +522,109 @@ Section ILEMMAS.
     des. subst. rewrite <- GRA.embed_add.
     rewrite <- URA.add_assoc. et.
   Qed.
+  Lemma IUpd_unfold I P
+  :
+  #=(I)=> P ⊢ (I -* #=> (I ** P)).
+Proof.
+  reflexivity.
+Qed.
 
+Lemma IUpd_fold I P
+  :
+  (I -* #=> (I ** P)) ⊢ #=(I)=> P.
+Proof.
+  reflexivity.
+Qed.
+
+Definition SubIProp P Q: iProp :=
+  Q -* #=> (P ** (P -* #=> Q)).
+
+Lemma SubIProp_refl P
+  :
+  ⊢ SubIProp P P.
+Proof.
+  iIntros "H". iFrame. auto.
+Qed.
+
+Lemma SubIProp_trans P Q R
+  :
+  (SubIProp P Q)
+    -∗
+    (SubIProp Q R)
+    -∗
+    (SubIProp P R).
+Proof.
+  iIntros "H0 H1 H2".
+  iPoseProof ("H1" with "H2") as "> [H1 H2]".
+  iPoseProof ("H0" with "H1") as "> [H0 H1]".
+  iFrame. iModIntro. iIntros "H".
+  iPoseProof ("H1" with "H") as "> H".
+  iPoseProof ("H2" with "H") as "H". auto.
+Qed.
+
+Lemma SubIProp_sep_l P Q
+  :
+  ⊢ (SubIProp P (P ** Q)).
+Proof.
+  iIntros "[H0 H1]". iFrame. auto.
+Qed.
+
+Lemma SubIProp_sep_r P Q
+  :
+  ⊢ (SubIProp Q (P ** Q)).
+Proof.
+  iIntros "[H0 H1]". iFrame. auto.
+Qed.
+
+Lemma IUpd_sub_mon P Q R
+  :
+  (SubIProp P Q)
+    -∗
+    (#=(P)=> R)
+    -∗
+    (#=(Q)=> R).
+Proof.
+  iIntros "H0 H1 H2".
+  iPoseProof (IUpd_unfold with "H1") as "H1".
+  iPoseProof ("H0" with "H2") as "> [H0 H2]".
+  iPoseProof ("H1" with "H0") as "> [H0 H1]".
+  iPoseProof ("H2" with "H0") as "H0". iFrame. auto.
+Qed.
 End ILEMMAS.
+Global Instance upd_elim_iupd `{GRA.t} I P Q
+       `{ElimModal _ True false false (#=(I)=> P) P Q R}
+  :
+  ElimModal True false false (#=> P) P Q R.
+Proof.
+  unfold ElimModal. i. iIntros "[H0 H1]".
+  iPoseProof (Upd_IUpd with "H0") as "> H0". iApply "H1". auto.
+Qed.
+
+Global Instance iupd_elim_upd `{GRA.t} I P Q b
+  :
+  ElimModal True b false (#=> P) P (#=(I)=> Q) (#=(I)=> Q).
+Proof.
+  unfold ElimModal. i. iIntros "[H0 H1]".
+  iPoseProof (Upd_IUpd with "H0") as "H0".
+  iIntros "H". iPoseProof ("H0" with "H") as "> [H0 H2]".
+  destruct b; ss.
+  { iPoseProof ("H2") as "# > H2". iPoseProof ("H1" with "H2") as "H".
+    iApply ("H" with "H0").
+  }
+  { iPoseProof ("H2") as "> H2". iPoseProof ("H1" with "H2") as "H".
+    iApply ("H" with "H0").
+  }
+Qed.
+
+Global Instance subiprop_elim_upd `{GRA.t} I J P Q b
+  :
+  ElimModal True b false ((SubIProp I J) ∗ #=(I)=> P) P (#=(J)=> Q) (#=(J)=> Q).
+Proof.
+  rewrite /ElimModal bi.intuitionistically_if_elim.
+  iIntros (_) "[[SUB P] K] J".
+  iMod ("SUB" with "J") as "[I IJ]". iMod ("P" with "I") as "[I P]".
+  iMod ("IJ" with "I") as "J". iPoseProof ("K" with "P J") as "K". iFrame.
+Qed.
 
 Ltac iOwnWf' H :=
   iPoseProof (OwnM_valid with H) as "%".
